boogie/red-black-tree/impact-sets.bpl
@@ -1,0 +1,187 @@
+// Supporting Artifact for
+// "Predictive Verification using Intrinsic Definitions of Data Structures"
+// by Adithya Murali, Cody Rivera, and P. Madhusudan.
+// 
+// Artifact by Cody Rivera, 2023. 
+//
+// Impact set verification for Red-Black trees.
+
+procedure Check_Set_k(x: Ref, arb: Ref, k: int)
+    modifies C.k;
+{
+    assume x != null;
+    assume LC(C.k, C.l, C.r, C.p, 
+              C.min, C.max, C.keys,
+              C.repr, C.black, C.black_height, 
+              arb, alloc);
+    assume arb != null;
+    assume arb != x;
+    assume arb != C.p[x];
+    C.k := C.k[x := k];
+    assert LC(C.k, C.l, C.r, C.p, 
+              C.min, C.max, C.keys,
+              C.repr, C.black, C.black_height, 
+              arb, alloc);
+}
+
+procedure Check_Set_l(x: Ref, arb: Ref, l: Ref)
+    modifies C.l;
+{
+    assume x != null;
+    assume LC(C.k, C.l, C.r, C.p, 
+              C.min, C.max, C.keys,
+              C.repr, C.black, C.black_height, 
+              arb, alloc);
+    assume arb != null;
+    assume arb != x;
+    assume arb != C.l[x];
+    C.l := C.l[x := l];
+    assert LC(C.k, C.l, C.r, C.p, 
+              C.min, C.max, C.keys,
+              C.repr, C.black, C.black_height, 
+              arb, alloc);
+}
+
+procedure Check_Set_r(x: Ref, arb: Ref, r: Ref)
+    modifies C.r;
+{
+    assume x != null;
+    assume LC(C.k, C.l, C.r, C.p, 
+              C.min, C.max, C.keys,
+              C.repr, C.black, C.black_height, 
+              arb, alloc);
+    assume arb != null;
+    assume arb != x;
+    assume arb != C.r[x];
+    C.r := C.r[x := r];
+    assert LC(C.k, C.l, C.r, C.p, 
+              C.min, C.max, C.keys,
+              C.repr, C.black, C.black_height, 
+              arb, alloc);
+}
+
+procedure Check_Set_p(x: Ref, arb: Ref, p: Ref)
+    modifies C.p;
+{
+    assume x != null;
+    assume LC(C.k, C.l, C.r, C.p, 
+              C.min, C.max, C.keys,
+              C.repr, C.black, C.black_height, 
+              arb, alloc);
+    assume arb != null;
+    assume arb != x;
+    assume arb != C.p[x];
+    C.p := C.p[x := p];
+    assert LC(C.k, C.l, C.r, C.p, 
+              C.min, C.max, C.keys,
+              C.repr, C.black, C.black_height, 
+              arb, alloc);
+}
+
+procedure Check_Set_min(x: Ref, arb: Ref, min: int)
+    modifies C.min;
+{
+    assume x != null;
+    assume LC(C.k, C.l, C.r, C.p, 
+              C.min, C.max, C.keys,
+              C.repr, C.black, C.black_height, 
+              arb, alloc);
+    assume arb != null;
+    assume arb != x;
+    assume arb != C.p[x];
+    C.min := C.min[x := min];
+    assert LC(C.k, C.l, C.r, C.p, 
+              C.min, C.max, C.keys,
+              C.repr, C.black, C.black_height, 
+              arb, alloc);
+}
+
+procedure Check_Set_max(x: Ref, arb: Ref, max: int)
+    modifies C.max;
+{
+    assume x != null;
+    assume LC(C.k, C.l, C.r, C.p, 
+              C.min, C.max, C.keys,
+              C.repr, C.black, C.black_height, 
+              arb, alloc);
+    assume arb != null;
+    assume arb != x;
+    assume arb != C.p[x];
+    C.max := C.max[x := max];
+    assert LC(C.k, C.l, C.r, C.p, 
+              C.min, C.max, C.keys,
+              C.repr, C.black, C.black_height, 
+              arb, alloc);
+}
+
+procedure Check_Set_keys(x: Ref, arb: Ref, keys: KeySet)
+    modifies C.keys;
+{
+    assume x != null;
+    assume LC(C.k, C.l, C.r, C.p, 
+              C.min, C.max, C.keys,
+              C.repr, C.black, C.black_height, 
+              arb, alloc);
+    assume arb != null;
+    assume arb != x;
+    assume arb != C.p[x];
+    C.keys := C.keys[x := keys];
+    assert LC(C.k, C.l, C.r, C.p, 
+              C.min, C.max, C.keys,
+              C.repr, C.black, C.black_height, 
+              arb, alloc);
+}
+
+procedure Check_Set_repr(x: Ref, arb: Ref, repr: RefSet)
+    modifies C.repr;
+{
+    assume x != null;
+    assume LC(C.k, C.l, C.r, C.p, 
+              C.min, C.max, C.keys,
+              C.repr, C.black, C.black_height, 
+              arb, alloc);
+    assume arb != null;
+    assume arb != x;
+    assume arb != C.p[x];
+    C.repr := C.repr[x := repr];
+    assert LC(C.k, C.l, C.r, C.p, 
+              C.min, C.max, C.keys,
+              C.repr, C.black, C.black_height, 
+              arb, alloc);
+}
+
+procedure Check_Set_black(x: Ref, arb: Ref, black: bool)
+    modifies C.black;
+{
+    assume x != null;
+    assume LC(C.k, C.l, C.r, C.p, 
+              C.min, C.max, C.keys,
+              C.repr, C.black, C.black_height, 
+              arb, alloc);
+    assume arb != null;
+    assume arb != x;
+    assume arb != C.p[x];
+    C.black := C.black[x := black];
+    assert LC(C.k, C.l, C.r, C.p, 
+              C.min, C.max, C.keys,
+              C.repr, C.black, C.black_height, 
+              arb, alloc);
+}
+
+procedure Check_Set_black_height(x: Ref, arb: Ref, black_height: int)
+    modifies C.black_height;
+{
+    assume x != null;
+    assume LC(C.k, C.l, C.r, C.p, 
+              C.min, C.max, C.keys,
+              C.repr, C.black, C.black_height, 
+              arb, alloc);
+    assume arb != null;
+    assume arb != x;
+    assume arb != C.p[x];
+    C.black_height := C.black_height[x := black_height];
+    assert LC(C.k, C.l, C.r, C.p, 
+              C.min, C.max, C.keys,
+              C.repr, C.black, C.black_height, 
+              arb, alloc);
+}
