boogie/red-black-tree/insert.bpl
@@ -34,7 +34,7 @@ procedure RBTInsertContract(x: Ref, k: int)
                 && C.min[ret] == k
                 && C.max[ret] == k
                 && C.black_height[ret] == 0
-                && fresh(C.repr[ret], alloc, old(alloc))
+                && Fresh(C.repr[ret], alloc, old(alloc))
                 && RefSetSubset(Br, EmptyRefSet[ret := true]));
     ensures (x != null ==>
                 KeySetsEqual(C.keys[ret], (old(C.keys)[x])[k := true])
@@ -44,6 +44,601 @@ procedure RBTInsertContract(x: Ref, k: int)
                 && (C.black[ret] ||
                         (!C.black[ret] && ((C.l[ret] == null || C.black[C.l[ret]] || C.r[ret] == null || C.black[C.r[ret]])
                         && (!old(C.black)[x] || ((C.l[ret] == null || C.black[C.l[ret]]) && (C.r[ret] == null || C.black[C.r[ret]]))))))
-                && fresh(RefSetDiffF(C.repr[ret], old(C.repr)[x]), alloc, old(alloc))
+                && Fresh(RefSetDiffF(C.repr[ret], old(C.repr)[x]), alloc, old(alloc))
                 && (old(C.p)[x] == null ==> RefSetSubset(Br, EmptyRefSet[ret := true]))
                 && (old(C.p)[x] != null ==> RefSetSubset(Br, (EmptyRefSet[ret := true])[old(C.p)[x] := true])));
+    // Framing conditions.
+    ensures Frame_all(
+        C.k, C.l, C.r, C.p, 
+        C.min, C.max, C.keys,
+        C.repr, C.black, C.black_height,
+        old(C.k), old(C.l), old(C.r), old(C.p), 
+        old(C.min), old(C.max), old(C.keys),
+        old(C.repr), old(C.black), old(C.black_height),
+        if x == null then EmptyRefSet else old(C.repr)[x], old(alloc)
+    );
+
+procedure RBTInsert(x: Ref, k: int)
+    returns (ret: Ref)
+    requires Br == EmptyRefSet;
+    requires x != null ==> LC(C.k, C.l, C.r, C.p, 
+                              C.min, C.max, C.keys,
+                              C.repr, C.black, C.black_height, 
+                              x, alloc);
+    requires x != null ==> !(C.keys[x])[k];
+    modifies C.k, C.l, C.r, C.p, 
+        C.min, C.max, C.keys,
+        C.repr, C.black, C.black_height, Br, alloc;
+    ensures RefSetSubset(old(alloc), alloc);
+    ensures ret != null;
+    ensures (LC(C.k, C.l, C.r, C.p, 
+               C.min, C.max, C.keys,
+               C.repr, C.black, C.black_height, 
+               ret, alloc) ||
+             LC_Trans_RedRed(C.k, C.l, C.r, C.p, 
+               C.min, C.max, C.keys,
+               C.repr, C.black, C.black_height, 
+               ret, alloc));
+    ensures C.p[ret] == null;
+    ensures x != null && x != ret ==> C.p[x] != old(C.p)[x];
+    ensures (x == null ==>
+                KeySetsEqual(C.keys[ret], EmptyKeySet[k := true])
+                && C.min[ret] == k
+                && C.max[ret] == k
+                && C.black_height[ret] == 0
+                && Fresh(C.repr[ret], alloc, old(alloc))
+                && RefSetSubset(Br, EmptyRefSet[ret := true]));
+    ensures (x != null ==>
+                KeySetsEqual(C.keys[ret], (old(C.keys)[x])[k := true])
+                && (C.min[ret] == old(C.min)[x] || C.min[ret] == k)
+                && (C.max[ret] == old(C.max)[x] || C.max[ret] == k)
+                && C.black_height[ret] == old(C.black_height)[x]
+                && (C.black[ret] ||
+                        (!C.black[ret] && ((C.l[ret] == null || C.black[C.l[ret]] || C.r[ret] == null || C.black[C.r[ret]])
+                        && (!old(C.black)[x] || ((C.l[ret] == null || C.black[C.l[ret]]) && (C.r[ret] == null || C.black[C.r[ret]]))))))
+                && Fresh(RefSetDiffF(C.repr[ret], old(C.repr)[x]), alloc, old(alloc))
+                && (old(C.p)[x] == null ==> RefSetSubset(Br, EmptyRefSet[ret := true]))
+                && (old(C.p)[x] != null ==> RefSetSubset(Br, (EmptyRefSet[ret := true])[old(C.p)[x] := true])));
+    // Framing conditions.
+    ensures Frame_all(
+        C.k, C.l, C.r, C.p, 
+        C.min, C.max, C.keys,
+        C.repr, C.black, C.black_height,
+        old(C.k), old(C.l), old(C.r), old(C.p), 
+        old(C.min), old(C.max), old(C.keys),
+        old(C.repr), old(C.black), old(C.black_height),
+        if x == null then EmptyRefSet else old(C.repr)[x], old(alloc)
+    );
+{
+    // Local variable declarations
+    var p: Ref;
+    var pl: Ref;
+    var pr: Ref;
+    var pll: Ref;
+    var plr: Ref;
+    var prl: Ref;
+    var prr: Ref;
+    var xl: Ref;
+    var xr: Ref;
+    var oldl: Ref;
+    var oldr: Ref;
+    var leaf: Ref;
+
+    if (x == null) {
+        call leaf := Create(k);
+
+        call Set_black(leaf, false);
+        call Set_min(leaf, k);
+        call Set_max(leaf, k);
+        call Set_keys(leaf, EmptyKeySet[C.k[leaf] := true]);
+        call Set_repr(leaf, EmptyRefSet[leaf := true]);
+        call Set_black_height(leaf, 0);
+        
+        call AssertLCAndRemove(leaf);
+        ret := leaf;
+    } else {
+        if (k < C.k[x]) {
+            if (C.l[x] != null) {
+                call IfNotBr_ThenLC(C.l[x]);
+            }
+            if (C.r[x] != null) {
+                call IfNotBr_ThenLC(C.r[x]);
+            }
+
+            call p := RBTInsertContract(C.l[x], k);
+
+            if (C.l[x] != null && C.l[x] != p) {
+                call IfNotBr_ThenLC(C.l[x]);
+            }
+            if (C.r[x] != null) {
+                call IfNotBr_ThenLC(C.r[x]);
+            }
+
+            if (C.black[p]) {
+                // assert {:split_here} true;
+                oldl := C.l[x];
+                call Set_l(x, p);
+                call Set_p(p, x);
+
+                call Set_min(x, if C.l[x] == null then C.k[x] else C.min[C.l[x]]);
+                call Set_max(x, if C.r[x] == null then C.k[x] else C.max[C.r[x]]);
+                call Set_keys(x, 
+                    KeySetUnionF(
+                        (if C.l[x] == null then EmptyKeySet else C.keys[C.l[x]])[C.k[x] := true],
+                        if C.r[x] == null then EmptyKeySet else C.keys[C.r[x]]
+                    )
+                );
+                call Set_repr(x, 
+                    RefSetUnionF(
+                        (if C.l[x] == null then EmptyRefSet else C.repr[C.l[x]])[x := true],
+                        if C.r[x] == null then EmptyRefSet else C.repr[C.r[x]]
+                    )
+                );
+                call Set_p(x, null);
+
+                call AssertLCAndRemove(p);
+                call AssertLCAndRemove(oldl);
+                ret := x;
+            } else {
+                xr := C.r[x];
+
+                if (xr != null && !C.black[xr]) {
+                    oldl := C.l[x];
+
+                    call Set_l(x, p);
+                    call Set_p(p, x);
+
+                    call Set_min(x, if C.l[x] == null then C.k[x] else C.min[C.l[x]]);
+                    call Set_max(x, if C.r[x] == null then C.k[x] else C.max[C.r[x]]);
+                    call Set_keys(x, 
+                        KeySetUnionF(
+                            (if C.l[x] == null then EmptyKeySet else C.keys[C.l[x]])[C.k[x] := true],
+                            if C.r[x] == null then EmptyKeySet else C.keys[C.r[x]]
+                        )
+                    );
+                    call Set_repr(x, 
+                        RefSetUnionF(
+                            (if C.l[x] == null then EmptyRefSet else C.repr[C.l[x]])[x := true],
+                            if C.r[x] == null then EmptyRefSet else C.repr[C.r[x]]
+                        )
+                    );
+                    call Set_p(x, null);
+
+                    call Set_black(x, false);
+                    call Set_black(p, true);
+                    call Set_black_height(p, C.black_height[p] + 1);
+                    call Set_black(xr, true);
+                    call Set_black_height(xr, C.black_height[xr] + 1);
+
+                    call AssertLCAndRemove(p);
+                    call AssertLCAndRemove(xr);
+                    call AssertLCAndRemove(oldl);
+
+                    ret := x;
+                } else {
+                    pl := C.l[p];
+                    pr := C.r[p];
+
+                    if (pl != null) {
+                        call IfNotBr_ThenLC(pl);
+                    }
+                    if (pr != null) {
+                        call IfNotBr_ThenLC(pr);
+                    }
+
+                    if (pr != null && !C.black[pr]) {
+                        assert {:focus} true;
+                        prl := C.l[pr];
+                        prr := C.r[pr];
+                        if (prl != null) {
+                            call IfNotBr_ThenLC(prl);
+                        }
+                        if (prr != null) {
+                            call IfNotBr_ThenLC(prr);
+                        }
+
+                        call Set_r(p, prl);
+                        if (prl != null) {
+                            call Set_p(prl, p);
+                        }
+                        oldl := C.l[x];
+                        call Set_l(x, prr);
+                        if (prr != null) {
+                            call Set_p(prr, x);
+                        }
+                        call Set_l(pr, p);
+                        call Set_p(p, pr);
+                        call Set_r(pr, x);
+                        call Set_p(x, pr);
+                        call Set_p(pr, null);
+
+                        call Set_min(p, if C.l[p] == null then C.k[p] else C.min[C.l[p]]);
+                        call Set_max(p, if C.r[p] == null then C.k[p] else C.max[C.r[p]]);
+                        call Set_keys(p, 
+                            KeySetUnionF(
+                                (if C.l[p] == null then EmptyKeySet else C.keys[C.l[p]])[C.k[p] := true],
+                                if C.r[p] == null then EmptyKeySet else C.keys[C.r[p]]
+                            )
+                        );
+                        call Set_repr(p, 
+                            RefSetUnionF(
+                                (if C.l[p] == null then EmptyRefSet else C.repr[C.l[p]])[p := true],
+                                if C.r[p] == null then EmptyRefSet else C.repr[C.r[p]]
+                            )
+                        );
+
+                        call Set_min(x, if C.l[x] == null then C.k[x] else C.min[C.l[x]]);
+                        call Set_max(x, if C.r[x] == null then C.k[x] else C.max[C.r[x]]);
+                        call Set_keys(x, 
+                            KeySetUnionF(
+                                (if C.l[x] == null then EmptyKeySet else C.keys[C.l[x]])[C.k[x] := true],
+                                if C.r[x] == null then EmptyKeySet else C.keys[C.r[x]]
+                            )
+                        );
+                        call Set_repr(x, 
+                            RefSetUnionF(
+                                (if C.l[x] == null then EmptyRefSet else C.repr[C.l[x]])[x := true],
+                                if C.r[x] == null then EmptyRefSet else C.repr[C.r[x]]
+                            )
+                        );
+                        if (C.black[x]) {
+                            call Set_black_height(x, C.black_height[x] - 1);
+                        }
+                        call Set_black(x, false);
+
+                        call Set_min(pr, if C.l[pr] == null then C.k[pr] else C.min[C.l[pr]]);
+                        call Set_max(pr, if C.r[pr] == null then C.k[pr] else C.max[C.r[pr]]);
+                        call Set_keys(pr, 
+                            KeySetUnionF(
+                                (if C.l[pr] == null then EmptyKeySet else C.keys[C.l[pr]])[C.k[pr] := true],
+                                if C.r[pr] == null then EmptyKeySet else C.keys[C.r[pr]]
+                            )
+                        );
+                        call Set_repr(pr, 
+                            RefSetUnionF(
+                                (if C.l[pr] == null then EmptyRefSet else C.repr[C.l[pr]])[pr := true],
+                                if C.r[pr] == null then EmptyRefSet else C.repr[C.r[pr]]
+                            )
+                        ); 
+                        call Set_black(pr, true);
+                        call Set_black_height(pr, C.black_height[pr] + 1);
+
+                        call AssertLCAndRemove(prl);
+                        call AssertLCAndRemove(prr);
+                        call AssertLCAndRemove(p);
+                        call AssertLCAndRemove(x);
+                        call AssertLCAndRemove(oldl);
+
+                        ret := pr;
+                    } else if (pl != null && !C.black[pl]) {
+                        assert {:focus} true;
+                        call Set_r(p, x);
+                        call Set_p(x, p);
+                        oldl := C.l[x];
+                        call Set_l(x, pr);
+                        if (pr != null) {
+                            call Set_p(pr, x);
+                        }
+                        call Set_p(p, null);
+
+                        call Set_min(x, if C.l[x] == null then C.k[x] else C.min[C.l[x]]);
+                        call Set_max(x, if C.r[x] == null then C.k[x] else C.max[C.r[x]]);
+                        call Set_keys(x, 
+                            KeySetUnionF(
+                                (if C.l[x] == null then EmptyKeySet else C.keys[C.l[x]])[C.k[x] := true],
+                                if C.r[x] == null then EmptyKeySet else C.keys[C.r[x]]
+                            )
+                        );
+                        call Set_repr(x, 
+                            RefSetUnionF(
+                                (if C.l[x] == null then EmptyRefSet else C.repr[C.l[x]])[x := true],
+                                if C.r[x] == null then EmptyRefSet else C.repr[C.r[x]]
+                            )
+                        );
+                        if (C.black[x]) {
+                            call Set_black_height(x, C.black_height[x] - 1);
+                        }
+                        call Set_black(x, false);
+
+                        call Set_min(p, if C.l[p] == null then C.k[p] else C.min[C.l[p]]);
+                        call Set_max(p, if C.r[p] == null then C.k[p] else C.max[C.r[p]]);
+                        call Set_keys(p, 
+                            KeySetUnionF(
+                                (if C.l[p] == null then EmptyKeySet else C.keys[C.l[p]])[C.k[p] := true],
+                                if C.r[p] == null then EmptyKeySet else C.keys[C.r[p]]
+                            )
+                        );
+                        call Set_repr(p, 
+                            RefSetUnionF(
+                                (if C.l[p] == null then EmptyRefSet else C.repr[C.l[p]])[p := true],
+                                if C.r[p] == null then EmptyRefSet else C.repr[C.r[p]]
+                            )
+                        );
+                        call Set_black(p, true);
+                        call Set_black_height(p, C.black_height[p] + 1);
+
+                        call AssertLCAndRemove(pr);
+                        call AssertLCAndRemove(x);
+                        call AssertLCAndRemove(oldl);
+
+                        ret := p;
+                    } else {
+                        // assert {:split_here} true;
+                        oldl := C.l[x];
+                        call Set_l(x, p);
+                        call Set_p(p, x);
+
+                        call Set_min(x, if C.l[x] == null then C.k[x] else C.min[C.l[x]]);
+                        call Set_max(x, if C.r[x] == null then C.k[x] else C.max[C.r[x]]);
+                        call Set_keys(x, 
+                            KeySetUnionF(
+                                (if C.l[x] == null then EmptyKeySet else C.keys[C.l[x]])[C.k[x] := true],
+                                if C.r[x] == null then EmptyKeySet else C.keys[C.r[x]]
+                            )
+                        );
+                        call Set_repr(x, 
+                            RefSetUnionF(
+                                (if C.l[x] == null then EmptyRefSet else C.repr[C.l[x]])[x := true],
+                                if C.r[x] == null then EmptyRefSet else C.repr[C.r[x]]
+                            )
+                        );
+                        call Set_p(x, null);
+
+                        call AssertLCAndRemove(p);
+                        call AssertLCAndRemove(oldl);
+                        ret := x;
+                    }
+                }
+            }
+        } else {
+            if (C.l[x] != null) {
+                call IfNotBr_ThenLC(C.l[x]);
+            }
+            if (C.r[x] != null) {
+                call IfNotBr_ThenLC(C.r[x]);
+            }
+
+            call p := RBTInsertContract(C.r[x], k);
+
+            if (C.l[x] != null) {
+                call IfNotBr_ThenLC(C.l[x]);
+            }
+            if (C.r[x] != null && C.r[x] != p) {
+                call IfNotBr_ThenLC(C.r[x]);
+            }
+
+            if (C.black[p]) {
+                oldr := C.r[x];
+                call Set_r(x, p);
+                call Set_p(p, x);
+
+                call Set_min(x, if C.l[x] == null then C.k[x] else C.min[C.l[x]]);
+                call Set_max(x, if C.r[x] == null then C.k[x] else C.max[C.r[x]]);
+                call Set_keys(x, 
+                    KeySetUnionF(
+                        (if C.l[x] == null then EmptyKeySet else C.keys[C.l[x]])[C.k[x] := true],
+                        if C.r[x] == null then EmptyKeySet else C.keys[C.r[x]]
+                    )
+                );
+                call Set_repr(x, 
+                    RefSetUnionF(
+                        (if C.l[x] == null then EmptyRefSet else C.repr[C.l[x]])[x := true],
+                        if C.r[x] == null then EmptyRefSet else C.repr[C.r[x]]
+                    )
+                );
+                call Set_p(x, null);
+
+                call AssertLCAndRemove(p);
+                call AssertLCAndRemove(oldr);
+                ret := x;
+            } else {
+                xl := C.l[x];
+
+                if (xl != null && !C.black[xl]) {
+                    oldr := C.r[x];
+                    call Set_r(x, p);
+                    call Set_p(p, x);
+
+                    call Set_min(x, if C.l[x] == null then C.k[x] else C.min[C.l[x]]);
+                    call Set_max(x, if C.r[x] == null then C.k[x] else C.max[C.r[x]]);
+                    call Set_keys(x, 
+                        KeySetUnionF(
+                            (if C.l[x] == null then EmptyKeySet else C.keys[C.l[x]])[C.k[x] := true],
+                            if C.r[x] == null then EmptyKeySet else C.keys[C.r[x]]
+                        )
+                    );
+                    call Set_repr(x, 
+                        RefSetUnionF(
+                            (if C.l[x] == null then EmptyRefSet else C.repr[C.l[x]])[x := true],
+                            if C.r[x] == null then EmptyRefSet else C.repr[C.r[x]]
+                        )
+                    );
+                    call Set_p(x, null);
+
+                    call Set_black(x, false);
+                    call Set_black(p, true);
+                    call Set_black_height(p, C.black_height[p] + 1);
+                    call Set_black(xl, true);
+                    call Set_black_height(xl, C.black_height[xl] + 1);
+
+                    call AssertLCAndRemove(p);
+                    call AssertLCAndRemove(xl);
+                    call AssertLCAndRemove(oldr);
+                    ret := x;
+                } else {
+                    pl := C.l[p];
+                    pr := C.r[p];
+
+                    if (pl != null) {
+                        call IfNotBr_ThenLC(pl);
+                    }
+                    if (pr != null) {
+                        call IfNotBr_ThenLC(pr);
+                    }
+
+                    if (pl != null && !C.black[pl]) {
+                        assert {:focus} true;
+                        pll := C.l[pl];
+                        plr := C.r[pl];
+                        if (pll != null) {
+                            call IfNotBr_ThenLC(pll);
+                        }
+                        if (plr != null) {
+                            call IfNotBr_ThenLC(plr);
+                        }
+
+                        call Set_l(p, plr);
+                        if (plr != null) {
+                            call Set_p(plr, p);
+                        }
+                        oldr := C.r[x];
+                        call Set_r(x, pll);
+                        if (pll != null) {
+                            call Set_p(pll, x);
+                        }
+                        call Set_r(pl, p);
+                        call Set_p(p, pl);
+                        call Set_l(pl, x);
+                        call Set_p(x, pl);
+                        call Set_p(pl, null);
+
+                        call Set_min(p, if C.l[p] == null then C.k[p] else C.min[C.l[p]]);
+                        call Set_max(p, if C.r[p] == null then C.k[p] else C.max[C.r[p]]);
+                        call Set_keys(p, 
+                            KeySetUnionF(
+                                (if C.l[p] == null then EmptyKeySet else C.keys[C.l[p]])[C.k[p] := true],
+                                if C.r[p] == null then EmptyKeySet else C.keys[C.r[p]]
+                            )
+                        );
+                        call Set_repr(p, 
+                            RefSetUnionF(
+                                (if C.l[p] == null then EmptyRefSet else C.repr[C.l[p]])[p := true],
+                                if C.r[p] == null then EmptyRefSet else C.repr[C.r[p]]
+                            )
+                        );
+
+                        call Set_min(x, if C.l[x] == null then C.k[x] else C.min[C.l[x]]);
+                        call Set_max(x, if C.r[x] == null then C.k[x] else C.max[C.r[x]]);
+                        call Set_keys(x, 
+                            KeySetUnionF(
+                                (if C.l[x] == null then EmptyKeySet else C.keys[C.l[x]])[C.k[x] := true],
+                                if C.r[x] == null then EmptyKeySet else C.keys[C.r[x]]
+                            )
+                        );
+                        call Set_repr(x, 
+                            RefSetUnionF(
+                                (if C.l[x] == null then EmptyRefSet else C.repr[C.l[x]])[x := true],
+                                if C.r[x] == null then EmptyRefSet else C.repr[C.r[x]]
+                            )
+                        );
+                        if (C.black[x]) {
+                            call Set_black_height(x, C.black_height[x] - 1);
+                        }
+                        call Set_black(x, false);
+
+                        call Set_min(pl, if C.l[pl] == null then C.k[pl] else C.min[C.l[pl]]);
+                        call Set_max(pl, if C.r[pl] == null then C.k[pl] else C.max[C.r[pl]]);
+                        call Set_keys(pl, 
+                            KeySetUnionF(
+                                (if C.l[pl] == null then EmptyKeySet else C.keys[C.l[pl]])[C.k[pl] := true],
+                                if C.r[pl] == null then EmptyKeySet else C.keys[C.r[pl]]
+                            )
+                        );
+                        call Set_repr(pl, 
+                            RefSetUnionF(
+                                (if C.l[pl] == null then EmptyRefSet else C.repr[C.l[pl]])[pl := true],
+                                if C.r[pl] == null then EmptyRefSet else C.repr[C.r[pl]]
+                            )
+                        ); 
+                        call Set_black(pl, true);
+                        call Set_black_height(pl, C.black_height[pl] + 1);
+
+                        call AssertLCAndRemove(pll);
+                        call AssertLCAndRemove(plr);
+                        call AssertLCAndRemove(p);
+                        call AssertLCAndRemove(x);
+                        call AssertLCAndRemove(oldr);
+
+                        ret := pl;
+                    } else if (pr != null && !C.black[pr]) {
+                        assert {:focus} true;
+                        call Set_l(p, x);
+                        call Set_p(x, p);
+                        oldr := C.r[x];
+                        call Set_r(x, pl);
+                        if (pl != null) {
+                            call Set_p(pl, x);
+                        }
+                        call Set_p(p, null);
+
+                        call Set_min(x, if C.l[x] == null then C.k[x] else C.min[C.l[x]]);
+                        call Set_max(x, if C.r[x] == null then C.k[x] else C.max[C.r[x]]);
+                        call Set_keys(x, 
+                            KeySetUnionF(
+                                (if C.l[x] == null then EmptyKeySet else C.keys[C.l[x]])[C.k[x] := true],
+                                if C.r[x] == null then EmptyKeySet else C.keys[C.r[x]]
+                            )
+                        );
+                        call Set_repr(x, 
+                            RefSetUnionF(
+                                (if C.l[x] == null then EmptyRefSet else C.repr[C.l[x]])[x := true],
+                                if C.r[x] == null then EmptyRefSet else C.repr[C.r[x]]
+                            )
+                        );
+                        if (C.black[x]) {
+                            call Set_black_height(x, C.black_height[x] - 1);
+                        }
+                        call Set_black(x, false);
+
+                        call Set_min(p, if C.l[p] == null then C.k[p] else C.min[C.l[p]]);
+                        call Set_max(p, if C.r[p] == null then C.k[p] else C.max[C.r[p]]);
+                        call Set_keys(p, 
+                            KeySetUnionF(
+                                (if C.l[p] == null then EmptyKeySet else C.keys[C.l[p]])[C.k[p] := true],
+                                if C.r[p] == null then EmptyKeySet else C.keys[C.r[p]]
+                            )
+                        );
+                        call Set_repr(p, 
+                            RefSetUnionF(
+                                (if C.l[p] == null then EmptyRefSet else C.repr[C.l[p]])[p := true],
+                                if C.r[p] == null then EmptyRefSet else C.repr[C.r[p]]
+                            )
+                        );
+                        call Set_black(p, true);
+                        call Set_black_height(p, C.black_height[p] + 1);
+
+                        call AssertLCAndRemove(pl);
+                        call AssertLCAndRemove(x);
+                        call AssertLCAndRemove(oldr);
+                        
+                        ret := p;
+                    } else {
+                        oldr := C.r[x];
+                        call Set_r(x, p);
+                        call Set_p(p, x);
+                        
+                        call Set_min(x, if C.l[x] == null then C.k[x] else C.min[C.l[x]]);
+                        call Set_max(x, if C.r[x] == null then C.k[x] else C.max[C.r[x]]);
+                        call Set_keys(x, 
+                            KeySetUnionF(
+                                (if C.l[x] == null then EmptyKeySet else C.keys[C.l[x]])[C.k[x] := true],
+                                if C.r[x] == null then EmptyKeySet else C.keys[C.r[x]]
+                            )
+                        );
+                        call Set_repr(x, 
+                            RefSetUnionF(
+                                (if C.l[x] == null then EmptyRefSet else C.repr[C.l[x]])[x := true],
+                                if C.r[x] == null then EmptyRefSet else C.repr[C.r[x]]
+                            )
+                        );
+                        call Set_p(x, null);
+
+                        call AssertLCAndRemove(p);
+                        call AssertLCAndRemove(oldr);
+                        ret := x;
+                    }
+                }
+            }
+        }
+    }
+}
